README.md
@@ -1,4 +1,4 @@
 # coq-practice
 Practice and experimentation with the [Coq proof assistant](https://coq.inria.fr/).
 
-`stlc/`: Proves progress and preservation of the simply-typed lambda calculus.
+`stlc/`: Proves soundness of the simply-typed lambda calculus.
